\section{Wichtige Formeln}
	$\sin^2(b)+\cos^2(b)=1 \qquad \tan(b)=\frac{\sin(b)}{\cos(b)}$
	
	
\subsection{Funktionswerte fÃ¼r Winkelargumente}
	\renewcommand{\arraystretch}{1.5}
	\begin{minipage}{5cm}
		\begin{tabular}[c]{ |c|c||c|c|c| }
	    	\hline
			deg & rad & sin & cos & tan\\
			\hline
			0\symbol{23} & 0 & 0 & 1 & 0\\
			\hline
			30\symbol{23} & $\frac{\pi}{6}$ & $\frac{1}{2}$ & $\frac{\sqrt{3}}{2}$ &
			$\frac{\sqrt{3}}{3}$\\
			\hline
			45\symbol{23} & $\frac{\pi}{4}$ & $\frac{\sqrt{2}}{2}$ & $\frac{\sqrt{2}}{2}$
			& 1\\
			\hline
			60\symbol{23} & $\frac{\pi}{3}$ & $\frac{\sqrt{3}}{2}$ & $\frac{1}{2}$ &
			$\sqrt{3}$\\
			\hline			
		\end{tabular}			
	\end{minipage}
	\begin{minipage}{4.3cm}
		\begin{tabular}[c]{ |c|c||c|c|}
	    	\hline
			deg & rad & sin & cos\\
			\hline
			90\symbol{23} & $\frac{\pi}{2}$ & 1 & 0\\
			\hline	
			120\symbol{23} & $\frac{2\pi}{3}$ & $\frac{\sqrt{3}}{2}$ & $-\frac{1}{2}$ \\
			\hline
			135\symbol{23} & $\frac{3\pi}{4}$ & $\frac{\sqrt{2}}{2}$ & $-\frac{\sqrt{2}}{2}$\\
			\hline
			150\symbol{23} & $\frac{5\pi}{6}$ & $\frac{1}{2}$ & $-\frac{\sqrt{3}}{2}$\\
			\hline
		\end{tabular}			
	\end{minipage}
	\begin{minipage}{4.5cm}
		\begin{tabular}[c]{ |c|c||c|c| }
	    	\hline
			deg & rad & sin & cos\\
			\hline
			180\symbol{23} & $\pi$ & 0 & -1\\
			\hline	
			210\symbol{23} & $\frac{7\pi}{6}$ & $-\frac{1}{2}$ & $-\frac{\sqrt{3}}{2}$\\
			\hline
			225\symbol{23} & $\frac{5\pi}{4}$ & $-\frac{\sqrt{2}}{2}$ & $-\frac{\sqrt{2}}{2}$\\
			\hline
			240\symbol{23} & $\frac{4\pi}{3}$ & $-\frac{\sqrt{3}}{2}$ & $-\frac{1}{2}$\\
			\hline
		\end{tabular}			
	\end{minipage}
	\begin{minipage}{4.5cm}
		\begin{tabular}[c]{ |c|c||c|c| }
	    	\hline
			deg & rad & sin & cos\\
			\hline
			270\symbol{23} & $\frac{3\pi}{2}$ & -1 & 0\\
			\hline	
			300\symbol{23} & $\frac{5\pi}{3}$ & $-\frac{\sqrt{3}}{2}$ & $\frac{1}{2}$\\
			\hline
			315\symbol{23} & $\frac{7\pi}{4}$ & $-\frac{\sqrt{2}}{2}$ & $\frac{\sqrt{2}}{2}$\\
			\hline
			330\symbol{23} & $\frac{11\pi}{6}$ & $-\frac{1}{2}$ & $\frac{\sqrt{3}}{2}$\\
			\hline
		\end{tabular}			
	\end{minipage}
	\renewcommand{\arraystretch}{1}
	
\subsection{PeriodizitÃ¤t}
	$\cos(a+k\cdot2\pi)=\cos(a) \qquad \sin(a+k\cdot2\pi)=\sin(a) \qquad
	(k \in \mathbb{Z})$
	
\subsection{Quadrantenbeziehungen}
	\begin{tabbing}
    	xxxxxxxxxxxxxxxxxxxxxxxxxxxxxxxxxx \= \kill
	  	$\sin(-a)=-\sin(a)$ \> $\cos(-a)=\cos(a)$\\
		$\sin(\pi - a)=\sin(a)$ \> $\cos(\pi - a)=-\cos(a)$\\
		$\sin(\pi + a)=-\sin(a)$ \> $\cos(\pi +a)=-\cos(a)$\\
		$\sin\left(\frac{\pi}{2}-a \right)=\sin\left(\frac{\pi}{2}+a \right)=\cos(a)$ \>
		$\cos\left(\frac{\pi}{2}-a \right)=-\cos\left(\frac{\pi}{2}+a \right)=\sin(a)$  
    \end{tabbing}

	\subsection{Additionstheoreme}
		$\sin(a \pm b)=\sin(a) \cdot \cos(b) \pm \cos(a) \cdot \sin(b)$\\
		$\cos(a \pm b)=\cos(a) \cdot \cos(b) \mp \sin(a) \cdot \sin(b)$\\	
		$\tan(a \pm b)=\dfrac{\tan(a) \pm \tan(b)}{1 \mp \tan(a) \cdot \tan(b)}$
		
	\subsection{Doppel- und Halbwinkel}	
		$\sin(2a)=2\sin(a)\cos(a)$\\
		$\cos(2a)=\cos^2(a)-\sin^2(a)=2\cos^2(a)-1=1-2\sin^2(a)$\\
		$\cos^2 \left(\frac{a}{2}\right)=\frac{1+\cos(a)}{2} \qquad
		\sin^2 \left(\dfrac{a}{2}\right)=\frac{1-\cos(a)}{2}$
		
	\subsection{Produkte}
		$\sin(a)\sin(b)=\frac{1}{2}(\cos(a-b)-\cos(a+b))$\\
		$\cos(a)\cos(b)=\frac{1}{2}(\cos(a-b)+\cos(a+b))$\\
		$\sin(a)\cos(b)=\frac{1}{2}(\sin(a-b)+\sin(a+b))$
		
	\subsection{Summe und Differenz}
		$\sin(a)+\sin(b)=2 \cdot \sin \left(\frac{a+b}{2}\right) \cdot
		\cos\left(\frac{a-b}{2}\right)$\\
		$\sin(a)-\sin(b)=2 \cdot \sin \left(\frac{a-b}{2}\right) \cdot
		\cos\left(\frac{a+b}{2}\right)$\\
		$\cos(a)+\cos(b)=2 \cdot \cos \left(\frac{a+b}{2}\right) \cdot
		\cos\left(\frac{a-b}{2}\right)$\\
		$\cos(a)-\cos(b)=-2 \cdot \sin \left(\frac{a+b}{2}\right) \cdot
		\cos\left(\frac{a-b}{2}\right)$\\
		$\tan(a) \pm \tan(b)=\dfrac{\sin(a \pm b)}{\cos(a)\cos(b)}$		

\subsection{Diverses}
\begin{tabbing}
	xxxxxxxxxxxxxxxxxxxxxxxxxxxx \= xxxxxxxxxxxxxxxxxxxxxxxxxxxxxx \= \kill
 	$f'(z) = \lim \limits_{\Delta z \rightarrow 0} \frac{f(z + \Delta z) -
	f(z)}{\Delta z}$ \> $(a + b)^n = \sum_{k=0}^{n} \binom n k a^{n-k} \cdot b^k$ \>
	$(a \pm b)^3 =a^3 \pm  3 a^{2} b + 3 a b^2 \pm b^3 $\\ \\
	$x_{1,2} = \dfrac{-b \pm \sqrt{b^2 - 4ac}}{2a}$ \> $\binom n k = \dfrac{n!}{k!
	\cdot (n-k)!}$ \> $(a \pm b)^4 =a^4 \pm  4 a^{3} b + 6a^2b^2 \pm 4 a b^3 +
	b^4$\\
\end{tabbing}